HOL_To_IMP/Refinements/HOL_TCN_To_IMP_Temp.thy
@@ -1,0 +1,184 @@
+theory HOL_TCN_To_IMP_Temp
+  imports HOL_To_IMP_Primitives "IMP.HOL_TCN_Timing"
+begin
+
+
+  (* assumes inf: "\<exists>zh v. (f,reg) \<turnstile> (t,vs_b,vs_arg) \<Rightarrow>\<^bsup>zh\<^esup> v" *)
+
+(* definition "interp_time1 reg g vs_arg_g = T_f_from_reg reg g vs_arg_g" *)
+(* definition "interp_time reg = sum_map (\<lambda>(g, vs_arg_g). interp_time1 reg g vs_arg_g)" *)
+  (* assumes "f_imp = to_imp_tc_1 f_args ctxt r0 f" *)
+  (* assumes "set (special_regs f_args ctxt r t) \<subseteq> set stale" *)
+
+lemma lookups_eq_on: assumes "s = t on set xs" shows "lookups xs s = lookups xs t"
+  using assms by (simp add: eq_on_def)
+
+abbreviation "lookup_args ctxt g \<equiv> lookups (args_from_ctxt ctxt g)"
+
+definition "tinterp_time reg ctxt =
+  sum_map
+    (\<lambda>(g, vs_arg_g).
+      HOL_Nat_To_IMP.least_constant_IMP (com_from_ctxt ctxt g) (T_f_from_reg reg g o lookup_args ctxt g)
+      * interp_time1 reg g vs_arg_g)"
+
+definition "well_formed_comp f_args ctxt bs stale t \<longleftrightarrow>
+  tailrec t
+  \<and> set (reserved_regs f_args ctxt bs t) \<subseteq> set stale
+  \<and> distinct f_args
+  \<and> (\<forall>g \<in> set (h_calls t). distinct (args_from_ctxt ctxt g))"
+
+definition "well_encoded_comp f_args bs vs_arg vs_b s \<longleftrightarrow> lookups f_args s = vs_arg \<and> lookups bs s = vs_b"
+
+definition "called_correctness ctxt reg t \<longleftrightarrow> (\<forall>g \<in> set (h_calls t).
+    HOL_Nat_To_IMP.terminates_with_res_time_order_IMP
+      (com_from_ctxt ctxt g) (ret_from_ctxt ctxt g)
+      (f_from_reg reg g o lookup_args ctxt g) (T_f_from_reg reg g o lookup_args ctxt g))" (* can we replace f with existential ? *)
+
+
+lemma ttime_non_tail:
+  fixes c :: tcom
+  assumes "invar c"
+  assumes "f \<turnstile> (c,s1) \<Rightarrow>\<^bsup>z\<^esup> s2"
+  assumes "teval_to_tail s1 c None"
+  shows "ttime_to_tail s1 c z"
+  sorry (* TODO *)
+
+lemma non_tail_tailrec: "non_tail t \<Longrightarrow> tailrec t"
+  by (induction t) auto
+
+(* TODO: need assumption relating registry and context *)
+lemma compiler_correct_nt:
+  assumes "non_tail t"
+  assumes "well_formed_comp f_args ctxt bs stale t"
+  assumes "well_encoded_comp f_args bs vs_arg vs_b s"
+  obtains f z s' where
+    "f \<turnstile> (to_imp_tc f_args ctxt bs r stale t,s) \<Rightarrow>\<^bsup>z\<^esup> s'"
+    "s' r = eval_non_tail reg vs_b vs_arg t"
+    "s = s' on (Set.remove r (set stale))"
+  nitpick
+  sorry
+
+
+lemma
+  assumes compiler_correct_nt_: True
+  assumes "t_imp = to_imp_tc f_args ctxt bs r stale t"
+  assumes "well_formed_comp f_args ctxt bs stale t"
+  assumes "well_encoded_comp f_args bs vs_arg vs_b s"
+  assumes "called_correctness ctxt reg t"
+  shows "\<exists>k z.
+    ttime_to_tail s t_imp (k + z)
+    \<and> k \<le> tstruct_k t_imp
+    \<and> z \<le> tinterp_time reg ctxt (time_to_tail reg vs_b vs_arg t)"
+using assms(2-5) proof (induction t arbitrary: t_imp bs r stale vs_b s)
+  case (hLet t1 t2)
+  thm hLet.prems(1)[simplified]
+  thm hLet.IH(1) hLet.IH(2)
+
+  thm hLet.prems
+
+  let ?x_var = "fresh' stale ''Let.x''"
+  let ?t_imp1 = "to_imp_tc f_args ctxt bs ?x_var stale t1"
+
+  have wf1: "well_formed_comp f_args ctxt bs stale t1" using hLet.prems(2)
+    unfolding well_formed_comp_def using non_tail_tailrec apply auto apply (simp only: reserved_regs_def h_calls.simps map_append)
+    by auto
+  then obtain k1 z1 where k1z1:
+      "ttime_to_tail s ?t_imp1 (k1 + z1)"
+      "k1 \<le> tstruct_k ?t_imp1"
+      "z1 \<le> tinterp_time reg ctxt (time_to_tail reg vs_b vs_arg t1)"
+    using hLet.IH(1)[where t_imp = ?t_imp1 and s = s and bs = bs and vs_b = vs_b and r = ?x_var and stale = stale] hLet.prems
+    unfolding called_correctness_def by auto
+
+  have ob1: "non_tail t1" using hLet unfolding well_formed_comp_def by simp
+  have ob2: "well_encoded_comp f_args bs vs_arg vs_b s" using hLet by simp
+  obtain f y1 s1
+      where t1s1: "f \<turnstile> (?t_imp1,s) \<Rightarrow>\<^bsup>y1\<^esup> s1"
+      and s1_xvar: "s1 ?x_var = eval_non_tail reg vs_b vs_arg t1"
+      and s1: "s = s1 on (Set.remove ?x_var (set stale))"
+    using compiler_correct_nt[OF ob1 wf1 ob2, simplified] by blast
+
+  have "tailrec t1" using well_formed_comp_def wf1 by blast
+  then have inv: "invar ?t_imp1" using to_imp_invar by blast
+  have y1: "y1 = k1 + z1" using ttime_non_tail[OF inv t1s1] sorry (* ttime_to_tail for non-tail MUST INVESTIGATE AND WRITE LEMMA *)
+
+  let ?t_imp2 = "to_imp_tc f_args ctxt (?x_var # bs) r (?x_var # stale) t2"
+  have "tailrec t2" using hLet unfolding well_formed_comp_def by simp
+
+  have t2_1: "well_formed_comp f_args ctxt (?x_var # bs) (?x_var # stale) t2"
+    using hLet.prems(2) unfolding well_formed_comp_def apply auto sorry (* almost sub-term *)
+  have "set f_args \<subseteq> Set.remove ?x_var (set stale)" using fresh_not_in_stale
+    unfolding remove_def apply simp using hLet.prems(2) unfolding well_formed_comp_def reserved_regs_def by simp
+  then have t2_2_1: "lookups f_args s1 = vs_arg"
+    apply (subst lookups_eq_on[where s = s, symmetric])
+    using s1 apply blast using hLet.prems(3) unfolding well_encoded_comp_def by blast
+  have "set bs \<subseteq> Set.remove ?x_var (set stale)" using fresh_not_in_stale
+    unfolding remove_def apply simp using hLet.prems(2) unfolding well_formed_comp_def reserved_regs_def by simp
+  then have t2_2_2: "lookups (?x_var # bs) s1 = eval_non_tail reg vs_b vs_arg t1 # vs_b" apply auto
+    using s1_xvar apply blast
+    apply (subst lookups_eq_on[where s = s, symmetric])
+    using s1 apply blast using hLet.prems(3) unfolding well_encoded_comp_def by blast
+  from t2_2_1 t2_2_2 have t2_2: "well_encoded_comp f_args (?x_var # bs) vs_arg (eval_non_tail reg vs_b vs_arg t1 # vs_b) s1"
+    unfolding well_encoded_comp_def by simp
+  have t2_3: "called_correctness ctxt reg t2" using hLet.prems(4) unfolding called_correctness_def by auto
+  obtain k2 z2 where k2z2:
+      "ttime_to_tail s1 ?t_imp2 (k2 + z2)"
+      "k2 \<le> tstruct_k ?t_imp2"
+      "z2 \<le> tinterp_time reg ctxt (time_to_tail reg (eval_non_tail reg vs_b vs_arg t1 # vs_b) vs_arg t2)"
+    using hLet.IH(2)[where t_imp = ?t_imp2 and r = r and s = s1 and bs = "?x_var # bs"
+      and vs_b = "eval_non_tail reg vs_b vs_arg t1 # vs_b" and stale = "?x_var # stale", OF _ t2_1 t2_2 t2_3, simplified]
+    by blast
+
+  from t1s1 k2z2
+  have "ttime_to_tail s t_imp (y1 + (k2 + z2))" using hLet.prems(1) apply simp unfolding Let_def apply (rule ttime_to_tail.intros(3)) by auto
+  moreover have "y1 + (k2 + z2) = (k1 + k2) + (z1 + z2)" using y1 by linarith
+  moreover have "k1 + k2 \<le> tstruct_k t_imp" using hLet.prems(1) apply simp unfolding Let_def using k1z1 k2z2 by simp
+  moreover have "z1 + z2 \<le> tinterp_time reg ctxt (time_to_tail reg vs_b vs_arg (hLet t1 t2))"
+    apply simp using k1z1 k2z2 unfolding tinterp_time_def by simp
+
+  ultimately show ?case by auto
+
+    (* idea: - solve premises of IH for t1, get k1 and z1 as structural/functional times for compiled t1
+               AND use compiler correctness to obtain y1 and s1 as run time and updated state of compiled t1
+             - show y1 = k1 + z1 using ttime_to_tail non_tail lemma for compiled t1
+             - ... *)
+next
+  case (hLetBound n)
+  then have t_imp: "t_imp = tAssign r (A (V (bs ! n)))" by simp
+
+  from t_imp have k: "ttime_to_tail s t_imp (2 + 0)" using ttime_to_tail.intros by simp
+  from t_imp have z: "2 \<le> tstruct_k t_imp" by simp
+
+  from k z show ?case by blast
+next
+  case (hArg n)
+  then have t_imp: "t_imp = tAssign r (A (V (f_args ! n)))" by simp
+
+  from t_imp have k: "ttime_to_tail s t_imp (2 + 0)" using ttime_to_tail.intros by simp
+  from t_imp have z: "2 \<le> tstruct_k t_imp" by simp
+
+  from k z show ?case by blast
+next
+  case (hNumber n) (* then show ?case using ttime_to_tail.intros by fastforce *)
+  then have t_imp: "t_imp = tAssign r (A (N n))" by simp
+
+  from t_imp have k: "ttime_to_tail s t_imp (2 + 0)" using ttime_to_tail.intros by simp
+  from t_imp have z: "2 \<le> tstruct_k t_imp" by simp
+
+  from k z show ?case by blast
+next
+  case (hIf t1 t2 t3)
+  then show ?case sorry
+next
+  case (hCall g ts)
+  then show ?case sorry
+next
+  case (hTAIL ts)
+  then show ?case sorry
+qed
+
+lemma "\<exists>c. \<forall>s. tstruct_k t_imp + something \<le> c * interp_time reg (time_to_tail reg vs_b vs_arg t)" oops
+(* in fact, we can calculate c as the max of the structural-constant-factor and all T_f_const-ants or so *)
+
+
+
+end
